src/Compiler.v
@@ -1,50 +1,28 @@
 Require Core Front RTL Flat CSE FirstOrder. 
 
 
-Definition compile Phi t  (a : forall Var, Front.action Phi Var t) : forall Var, Flat.block Phi Var t.  
-intros.
-apply Flat.compile. 
-apply RTL.nblock_to_block. 
-apply RTL.compile. 
-apply a. 
-Defined. 
+Definition Compile Phi t  (a : forall Var, Front.action Phi Var t) : Flat.Block Phi t :=
+  let x := RTL.Compile Phi  t a in
+  let x := Flat.Compile Phi t x in 
+  let x := CSE.Compile Phi t  x in  
+        x. 
 
-
-Lemma compile_correct (Phi : Core.state) t a :
-  let block := compile Phi t a in 
+Lemma Compile_correct (Phi : Core.state) t a :
+  let block := Compile Phi t a in 
   forall st Delta, 
-  Flat.eval_block Phi st t (block Core.eval_type) Delta =
-     Front.Sem.eval_action (a Core.eval_type) st Delta. 
-Proof. 
-  intros. 
-
-  rewrite <- RTL.CPS_compile_correct.        
-  rewrite <- RTL.nblock_compile_correct.
-  rewrite <- Flat.compile_correct. 
-  unfold block. unfold compile. 
+    Flat.Eval Phi st t block Delta =
+    Front.Eval Phi st t a Delta. 
+Proof.
+  unfold Compile. intros. 
+  rewrite CSE.Compile_correct. 
+  rewrite Flat.Compile_correct. 
+  rewrite RTL.Compile_correct. 
   reflexivity. 
+  admit. 
 Qed. 
 
-Print Assumptions compile_correct. 
+Print Assumptions Compile_correct. 
 
-Definition fo_compile Phi t  (a : forall Var, Front.action Phi Var t) :  FirstOrder.block Phi t.  
-intros.
-apply FirstOrder.compile. 
-apply Flat.compile. 
-apply RTL.nblock_to_block. 
-apply RTL.compile. 
-apply a. 
-Defined. 
-
-
-Definition fo_cse_compile Phi t  (a : forall Var, Front.action Phi Var t) :  FirstOrder.block Phi t.  
-intros.
-apply FirstOrder.compile. 
-apply CSE.cse_block. 
-apply Flat.compile. 
-apply RTL.nblock_to_block. 
-apply RTL.compile. 
-apply a. 
-Defined. 
-
-Print Opaque Dependencies fo_cse_compile.
+Definition Fo_compile Phi t (A : Front.Action Phi t) :  FirstOrder.block Phi t :=
+  let x := Compile Phi t A in 
+    FirstOrder.compile Phi t (x _ ).  
